src/ASN1/ASN1.Spec.Interpreter.fst
@@ -6,6 +6,8 @@ include LowParse.Spec.List
 include LowParse.Spec.Defaultable
 include LowParse.Spec.Bytes
 
+include ASN1.Debug
+
 open ASN1.Base
 open ASN1.Spec.Content.BOOLEAN
 open ASN1.Spec.Content.INTEGER
@@ -25,57 +27,112 @@ open ASN1.Spec.Any
 
 module List = FStar.List.Tot
 
-(*
+let rec dasn1_terminal_as_parser (k : asn1_terminal_k) : asn1_weak_parser (asn1_terminal_t k)  =
+  parse_debug #(asn1_terminal_t k) #(asn1_weak_parser_kind) "asn1_terminal_as_parser"
+  (match k with
+  | ASN1_BOOLEAN -> weaken _ parse_asn1_boolean
+  | ASN1_INTEGER -> weaken _ ((parse_untagged_bounded_integer 20) `parse_synth` (fun x -> x <: int))
+  | ASN1_BITSTRING -> parse_asn1_bitstring
+  | ASN1_OCTETSTRING -> parse_asn1_octetstring
+  | ASN1_UTF8STRING -> parse_asn1_utf8string
+  | ASN1_PRINTABLESTRING -> parse_asn1_printablestring
+  | ASN1_IA5STRING -> parse_asn1_ia5string
+  | ASN1_NULL -> parse_asn1_null
+  | ASN1_OID -> parse_asn1_OIDU32
+  | ASN1_UTCTIME -> parse_asn1_UTCTIME
+  | ASN1_GENERALIZEDTIME -> parse_asn1_GENERALIZEDTIME
+  | ASN1_PREFIXED_TERMINAL id k -> weaken asn1_weak_parser_kind (parse_asn1_ILC id #(ASN1_TERMINAL k) (dasn1_terminal_as_parser k)))
 
-let make_asn1_closed_any_OIDU32_parser
-  (id : asn1_id_t)
-  (ls : list (asn1_oid_t * asn1_gen_items_k))
-  (pf : squash((List.noRepeats (List.map fst ls))))
-  (k : asn1_content_k)
-  (lp : list (asn1_oid_t & (gen_parser asn1_weak_parser_kind)))
-: Pure (asn1_weak_parser (asn1_content_t k))
-  (requires ((k == ASN1_ANY_OID id ls None pf) /\ (asn1_any_t asn1_oid_t ls == extract_types lp)))
-  (ensures fun _ -> True)
-= weaken asn1_weak_parser_kind (make_gen_choice_weak_parser (parse_asn1_ILC id #(ASN1_TERMINAL ASN1_OID) parse_asn1_OIDU32) lp)
+and dasn1_content_as_parser (k : asn1_content_k) : Tot (asn1_weak_parser (asn1_content_t k)) (decreases k) =
+  match k with
+  | ASN1_RESTRICTED_TERMINAL k' is_valid -> weaken _ ((dasn1_terminal_as_parser k') `parse_filter` is_valid)
+  | ASN1_TERMINAL k' -> dasn1_terminal_as_parser k'
+  | ASN1_SEQUENCE gitems -> make_asn1_sequence_parser (dasn1_sequence_as_parser (dfst gitems))
+  | ASN1_SEQUENCE_OF k' -> weaken asn1_weak_parser_kind (parse_list (dasn1_as_parser k'))
+  | ASN1_SET_OF k' -> weaken _ (dasn1_as_parser k')
+  | ASN1_PREFIXED k' -> weaken _ (dasn1_as_parser k')
+  | ASN1_ANY_DEFINED_BY prefix id key_k ls ofb pf pf' -> 
+    let itemtwins = dasn1_sequence_as_parser prefix in
+    let key_p_twin = 
+      (let kc = ASN1_TERMINAL key_k in
+      let p = dasn1_terminal_as_parser key_k in
+      let _ = parser_asn1_ILC_twin_case_injective id #kc p in
+      Mkparsertwin #asn1_strong_parser_kind #(asn1_terminal_t key_k) (parse_asn1_ILC id #kc p) (parse_asn1_ILC_twin id #kc p))
+    in
+    let key_p = Mkparsertwin?.p key_p_twin in
+    let key_fp = Mkparsertwin?.fp key_p_twin in
+    let supported_p = dasn1_ls_as_parser (asn1_terminal_t key_k) ls in
+    (match ofb with
+    | None -> 
+      let suffix_p_twin = (Mkparsertwin #asn1_weak_parser_kind #(make_gen_choice_type (extract_types supported_p))
+        (weaken asn1_weak_parser_kind (make_gen_choice_weak_parser key_p supported_p))
+        (let _ = make_gen_choice_weak_parser_twin_and_then_cases_injective key_fp supported_p in
+         fun id -> weaken asn1_weak_parser_kind (make_gen_choice_weak_parser_twin key_fp supported_p id)))
+      in
+      make_asn1_sequence_any_parser itemtwins suffix_p_twin
+    | Some gitems -> 
+      let fallback_p = Mkgenparser _ (make_asn1_sequence_parser (dasn1_sequence_as_parser (dfst gitems))) in
+      let suffix_p_twin = (Mkparsertwin #asn1_weak_parser_kind #(make_gen_choice_type_with_fallback (extract_types supported_p) (Mkgenparser?.t fallback_p))
+        (weaken asn1_weak_parser_kind (make_gen_choice_with_fallback_weak_parser key_p supported_p fallback_p))
+        (let _ = make_gen_choice_with_fallback_weak_parser_twin_and_then_cases_injective key_fp supported_p fallback_p in
+         fun id -> weaken asn1_weak_parser_kind (make_gen_choice_with_fallback_weak_parser_twin key_fp supported_p fallback_p id))) 
+      in
+      make_asn1_sequence_any_parser itemtwins suffix_p_twin) 
 
-let make_asn1_closed_any_INTEGER_parser
-  (id : asn1_id_t)
-  (ls : list (asn1_integer_t * asn1_gen_items_k))
-  (pf : squash(List.noRepeats (List.map fst ls)))
-  (k : asn1_content_k)
-  (lp : list (asn1_integer_t & (gen_parser asn1_weak_parser_kind)))
-: Pure (asn1_weak_parser (asn1_content_t k))
-  (requires ((k == ASN1_ANY_INTEGER id ls None pf) /\ (asn1_any_t asn1_integer_t ls == extract_types lp)))
-  (ensures fun _ -> True)
-= weaken asn1_weak_parser_kind (make_gen_choice_weak_parser (parse_asn1_ILC id #(ASN1_TERMINAL ASN1_INTEGER) (weaken _ ((parse_untagged_bounded_integer 20) `parse_synth` (fun x -> x <: int)))) lp)
+and dasn1_ls_as_parser (t : eqtype) (ls : list (t * asn1_gen_items_k)) : Tot (lp : list (t & (gen_parser asn1_weak_parser_kind)) {asn1_any_t t ls == extract_types lp}) (decreases ls) =
+  match ls with
+  | [] -> [] 
+  | h :: tl -> 
+    let (x, y) = h in
+    (x, Mkgenparser _ (make_asn1_sequence_parser (dasn1_sequence_as_parser (dfst y)))) :: (dasn1_ls_as_parser t tl)
 
-let make_asn1_open_any_OIDU32_parser
-  (id : asn1_id_t)
-  (ls : list (asn1_oid_t * asn1_gen_items_k))
-  (fbk : asn1_gen_items_k)
-  (fbp : asn1_weak_parser (asn1_sequence_t (dfst fbk)))
-  (pf : squash((List.noRepeats (List.map fst ls))))
-  (k : asn1_content_k)
-  (lp : list (asn1_oid_t & (gen_parser asn1_weak_parser_kind)))
-: Pure (asn1_weak_parser (asn1_content_t k))
-  (requires ((k == ASN1_ANY_OID id ls (Some fbk) pf) /\ (asn1_any_t asn1_oid_t ls == extract_types lp)))
-  (ensures fun _ -> True)
-= weaken asn1_weak_parser_kind (make_gen_choice_with_fallback_weak_parser (parse_asn1_ILC id #(ASN1_TERMINAL ASN1_OID) parse_asn1_OIDU32) lp (Mkgenparser _ fbp))
+and dasn1_lc_as_parser (lc : list (asn1_id_t & asn1_content_k)) : Tot (lp : list (asn1_id_t & (gen_parser asn1_strong_parser_kind)) {asn1_lc_t lc == extract_types lp})  (decreases lc) =
+  match lc with
+  | [] -> [] 
+  | h :: t -> 
+    let (x, y) = h in
+    (x, Mkgenparser (asn1_content_t y) (parse_asn1_LC (dasn1_content_as_parser y))) :: (dasn1_lc_as_parser t)
 
-let make_asn1_open_any_INTEGER_parser
-  (id : asn1_id_t)
-  (ls : list (asn1_integer_t * asn1_gen_items_k))
-  (fbk : asn1_gen_items_k)
-  (fbp : asn1_weak_parser (asn1_sequence_t (dfst fbk)))
-  (pf : squash((List.noRepeats (List.map fst ls))))
-  (k : asn1_content_k)
-  (lp : list (asn1_integer_t & (gen_parser asn1_weak_parser_kind)))
-: Pure (asn1_weak_parser (asn1_content_t k))
-  (requires ((k == ASN1_ANY_INTEGER id ls (Some fbk) pf) /\ (asn1_any_t asn1_integer_t ls == extract_types lp)))
-  (ensures fun _ -> True)
-= weaken asn1_weak_parser_kind (make_gen_choice_with_fallback_weak_parser (parse_asn1_ILC id #(ASN1_TERMINAL ASN1_INTEGER) (weaken _ ((parse_untagged_bounded_integer 20) `parse_synth` (fun x -> x <: int)))) lp (Mkgenparser _ fbp))
+and dasn1_as_parser (#s : _) (k : asn1_k s) : Tot (asn1_strong_parser (asn1_t k)) (decreases k) =
+  match k with
+  | ASN1_ILC id k' -> parse_debug "ASN1_ILC" (parse_asn1_ILC id (dasn1_content_as_parser k'))
+  | ASN1_CHOICE_ILC lc pf -> parse_debug "ASN1_CHOICE" (make_asn1_choice_parser lc pf k (dasn1_lc_as_parser lc))
+  | ASN1_ANY_ILC -> parse_asn1_anyILC
 
-*)
+and dasn1_as_parser_twin (#s : _) (k : asn1_k s) : Tot (asn1_strong_parser (asn1_t k) & (fp : (asn1_id_t -> asn1_strong_parser (asn1_t k)) {and_then_cases_injective fp})) (decreases k) =
+  match k with
+  | ASN1_ILC id k' -> 
+    let p = dasn1_content_as_parser k' in
+    let _ = parser_asn1_ILC_twin_case_injective id p in
+    (parse_debug "ASN1_ILC" (parse_asn1_ILC id p), parse_asn1_ILC_twin id p)
+  | ASN1_CHOICE_ILC lc pf ->
+    let lp = dasn1_lc_as_parser lc in
+    let _ = make_asn1_choice_parser_twin_cases_injective lc pf k lp in
+    (parse_debug "ASN1_CHOICE" (make_asn1_choice_parser lc pf k lp), make_asn1_choice_parser_twin lc pf k lp)
+  | ASN1_ANY_ILC -> 
+    let _ = parse_asn1_anyILC_twin_and_then_cases_injective () in
+    (parse_asn1_anyILC, parse_asn1_anyILC_twin)
+
+and dasn1_decorated_as_parser_twin (item : asn1_gen_item_k) : Tot (gp : gen_decorated_parser_twin {Mkgendcparser?.d gp == item}) =
+  match item with
+  | (| _, _, dk |) -> match dk with
+                    | ASN1_PLAIN_ILC k -> 
+                      let (p, fp) = dasn1_as_parser_twin k in
+                      Mkgendcparser item p fp
+                    | ASN1_OPTION_ILC k -> 
+                      let (p, fp) = dasn1_as_parser_twin k in
+                      Mkgendcparser item p fp
+                    | ASN1_DEFAULT_TERMINAL id #k defv ->
+                      let p = dasn1_terminal_as_parser k in
+                      Mkgendcparser item (parse_asn1_ILC id #(ASN1_TERMINAL k) p) (parse_asn1_ILC_twin id #(ASN1_TERMINAL k) p)
+                    | ASN1_DEFAULT_RESTRICTED_TERMINAL id #k is_valid defv ->
+                      let p : asn1_weak_parser (asn1_decorated_pure_t item) = weaken _ ((dasn1_terminal_as_parser k) `parse_filter` is_valid) in
+                      Mkgendcparser item (parse_asn1_ILC id #(ASN1_RESTRICTED_TERMINAL k is_valid) p) (parse_asn1_ILC_twin id #(ASN1_RESTRICTED_TERMINAL k is_valid) p)
+
+and dasn1_sequence_as_parser (items : list asn1_gen_item_k) : Tot (lp : list gen_decorated_parser_twin {List.map (Mkgendcparser?.d) lp == items}) (decreases items) =
+  match items with
+  | [] -> []
+  | hd :: tl -> (dasn1_decorated_as_parser_twin hd) :: (dasn1_sequence_as_parser tl)
 
 let rec asn1_terminal_as_parser (k : asn1_terminal_k) : asn1_weak_parser (asn1_terminal_t k)  =
   match k with
@@ -100,7 +157,7 @@ and asn1_content_as_parser (k : asn1_content_k) : Tot (asn1_weak_parser (asn1_co
   | ASN1_SEQUENCE_OF k' -> weaken asn1_weak_parser_kind (parse_list (asn1_as_parser k'))
   | ASN1_SET_OF k' -> weaken _ (asn1_as_parser k')
   | ASN1_PREFIXED k' -> weaken _ (asn1_as_parser k')
-  | ASN1_ANY_DEFINED_BY prefix id key_k ls ofb pf_wf pf_sup -> 
+  | ASN1_ANY_DEFINED_BY prefix id key_k ls ofb pf pf' -> 
     let itemtwins = asn1_sequence_as_parser prefix in
     let key_p_twin = 
       (let kc = ASN1_TERMINAL key_k in
@@ -182,4 +239,4 @@ and asn1_sequence_as_parser (items : list asn1_gen_item_k) : Tot (lp : list gen_
   match items with
   | [] -> []
   | hd :: tl -> (asn1_decorated_as_parser_twin hd) :: (asn1_sequence_as_parser tl)
-  
+
