src/ASN1/ASN1.Debug.fsti
@@ -1,0 +1,20 @@
+module ASN1.Debug
+open LowParse.Spec.Base
+
+val parse_debug
+  (#t: Type)
+  (#k: parser_kind)
+  (msg: string)
+  (p: parser k t)
+: Pure (parser k t)
+    (requires True)
+    (ensures (fun f -> forall input . parse f input == parse p input))
+
+val print_debug
+  (#t: Type)
+  (msg: string)
+  (v: t)
+: Pure t
+    (requires True)
+    (ensures (fun v' -> v' == v))
+    
